Use the new let-operators instead of `<--`

fstar/MLS.Result.fst
@@ -2,44 +2,53 @@ module MLS.Result
 
 #set-options "--fuel 0 --ifuel 0"
 
-type result 'a =
-  | Success: v:'a -> result 'a
-  | InternalError: string -> result 'a
-  | ProtocolError: string -> result 'a
+type result (a:Type) =
+  | Success: v:a -> result a
+  | InternalError: string -> result a
+  | ProtocolError: string -> result a
 
-let return (a:'a) : result 'a = Success a
-let internal_failure (#a:Type) (s:string): result a = InternalError s
-let error (#a:Type) (s:string): result a = ProtocolError s
+val return: #a:Type -> a -> result a
+let return #a x = Success x
+
+val internal_failure: #a:Type -> s:string -> result a
+let internal_failure #a s = InternalError s
+
+val error: #a:Type -> s:string -> result a
+let error #a s = ProtocolError s
 
 #push-options "--ifuel 1"
 //TODO unfold? (to remove all the lambdas in the spec and in the generated code)
-let bind (a:result 'a) (f:'a -> result 'b) : result 'b =
-  match a with
+val (let?): #a:Type -> #b:Type -> result a -> (a -> result b) -> result b
+let (let?) #a #b rx f =
+  match rx with
   | Success x -> f x
   | InternalError x -> InternalError x
   | ProtocolError x -> ProtocolError x
 #pop-options
 
-let from_option (s:string) (x:option 'a): result 'a =
+val from_option: #a:Type -> string -> option a -> result a
+let from_option #a s x =
   match x with
   | None -> ProtocolError s
   | Some x -> Success x
 
 #push-options "--ifuel 1 --fuel 1"
-let rec mapM (f:('a -> result 'b)) (l:list 'a): result (res:list 'b{List.Tot.length res == List.Tot.length l}) =
+val mapM: #a:Type -> #b:Type -> (a -> result b) -> l:list a -> result (res:list b{List.Tot.length res == List.Tot.length l})
+let rec mapM #a #b f l =
   match l with
   | [] -> return []
   | h::t ->
-    fh <-- f h;
-    ft <-- mapM f t;
-    return #(res:list 'b{List.Tot.length res == List.Tot.length l}) (fh::ft)
+    let? fh = f h in
+    let? ft = mapM f t in
+    return #(res:list b{List.Tot.length res == List.Tot.length l}) (fh::ft)
 #pop-options
 
 #push-options "--ifuel 1 --fuel 1"
-let rec fold_leftM (f:'a -> 'b -> result 'a) (x:'a) (l:list 'b): Tot (result 'a) (decreases l) =
+val fold_leftM: #a:Type -> #b:Type -> (a -> b -> result a) -> a -> list b -> result a
+let rec fold_leftM #a #b f x l: Tot (result a) (decreases l) =
   match l with
   | [] -> return x
   | h::t ->
-    new_x <-- f x h;
+    let? new_x = f x h in
     fold_leftM f new_x t
 #pop-options
