fstar/MLS.fst
@@ -60,12 +60,12 @@ noeq type state = {
 #push-options "--fuel 1"
 val compute_group_context: #l:nat -> bytes -> nat -> treesync bytes #cb.base tkt l 0 -> bytes -> result (group_context_nt bytes)
 let compute_group_context #l group_id epoch tree confirmed_transcript_hash =
-  tree_hash <-- (
+  let? tree_hash = (
     if not (MLS.TreeSync.TreeHash.tree_hash_pre tree) then
       internal_failure "state_to_group_context: tree_hash precondition false"
     else
       return #bytes (MLS.TreeSync.TreeHash.tree_hash #bytes #cb tree)
-  );
+  ) in
   if not (length group_id < pow2 30) then
     internal_failure "state_to_group_context: group_id too long"
   else if not (epoch < pow2 64) then
@@ -103,10 +103,10 @@ let reset_ratchet_states st =
   if not (st.leaf_index < pow2 st.treesync_state.levels) then
      internal_failure "reset_ratchet_states: leaf_index too big"
   else (
-    encryption_secret <-- MLS.TreeDEM.Keys.secret_epoch_to_encryption st.epoch_secret;
-    leaf_secret <-- MLS.TreeDEM.Keys.leaf_kdf #bytes #bytes_crypto_bytes #st.treesync_state.levels #0 encryption_secret st.leaf_index;
-    handshake_state <-- MLS.TreeDEM.Keys.init_handshake_ratchet leaf_secret;
-    application_state <-- MLS.TreeDEM.Keys.init_application_ratchet leaf_secret;
+    let? encryption_secret = MLS.TreeDEM.Keys.secret_epoch_to_encryption st.epoch_secret in
+    let? leaf_secret = MLS.TreeDEM.Keys.leaf_kdf #bytes #bytes_crypto_bytes #st.treesync_state.levels #0 encryption_secret st.leaf_index in
+    let? handshake_state = MLS.TreeDEM.Keys.init_handshake_ratchet leaf_secret in
+    let? application_state = MLS.TreeDEM.Keys.init_application_ratchet leaf_secret in
     return ({st with handshake_state; application_state})
   )
 #pop-options
@@ -115,7 +115,7 @@ val process_proposal: nat -> state -> proposal bytes -> result state
 let process_proposal sender_id st p =
   match p with
   | Add key_package ->
-    add_pend <-- MLS.TreeSync.API.prepare_add st.treesync_state key_package;
+    let? add_pend = MLS.TreeSync.API.prepare_add st.treesync_state key_package in
     // TODO AS check
     let (treesync_state, _) = MLS.TreeSync.API.finalize_add add_pend () in
     assume (length #bytes key_package.tbs.leaf_node.data.content = hpke_public_key_length #bytes);
@@ -125,7 +125,7 @@ let process_proposal sender_id st p =
     if not (sender_id < pow2 st.treesync_state.levels) then
       error "process_proposal: leaf_ind is greater than treesize"
     else (
-      pend_update <-- MLS.TreeSync.API.prepare_update st.treesync_state leaf_package sender_id;
+      let? pend_update = MLS.TreeSync.API.prepare_update st.treesync_state leaf_package sender_id in
       // TODO AS check
       let treesync_state = MLS.TreeSync.API.finalize_update pend_update () in
       assume (length #bytes leaf_package.data.content = hpke_public_key_length #bytes);
@@ -138,7 +138,7 @@ let process_proposal sender_id st p =
       error "process_proposal: leaf_index too big"
     else (
       assume(st.treesync_state.levels == st.treekem_state.levels);
-      remove_pend <-- MLS.TreeSync.API.prepare_remove st.treesync_state leaf_index;
+      let? remove_pend = MLS.TreeSync.API.prepare_remove st.treesync_state leaf_index in
       let treesync_state = MLS.TreeSync.API.finalize_remove remove_pend in
       let treekem_state = MLS.TreeKEM.API.remove st.treekem_state leaf_index in
       return ({ st with treesync_state; treekem_state })
@@ -167,52 +167,52 @@ val process_commit: state -> msg:message_content bytes{msg.content_type = CT_com
 let process_commit state message message_auth =
   let message: MLS.TreeDEM.Message.Types.message_content bytes = message in
   let message_content: commit bytes = message.content in
-  sender_id <-- (
+  let? sender_id = (
     if not (S_member? message.sender) then
       error "process_commit: sender is not a member"
     else (
       return #nat (S_member?.leaf_index message.sender)
     )
-  );
+  ) in
   // 0. Process proposals
-  proposals <-- mapM (proposal_or_ref_to_proposal state) message_content.c_proposals;
-  state <-- process_proposals state sender_id proposals;
+  let? proposals = mapM (proposal_or_ref_to_proposal state) message_content.c_proposals in
+  let? state = process_proposals state sender_id proposals in
   // 1. Process update path
-  state <-- (
+  let? state = (
     match message_content.c_path with
     | None -> return state
     | Some path ->
-      group_context <-- state_to_group_context state;
+      let? group_context = state_to_group_context state in
       let group_context_bytes = (ps_to_pse ps_group_context_nt).serialize_exact group_context in
       //It is not possible to move this `if` inside the definition of `update_pathkem`, because we need the information it gives to write the type of `update_pathkem`
       if not (sender_id < pow2 state.treesync_state.levels) then
         error "process_commit: sender_id is greater than treesize"
       else (
         assume(state.treesync_state.levels == state.treekem_state.levels);
-        uncompressed_path <-- uncompress_update_path sender_id state.treesync_state.tree path;
+        let? uncompressed_path = uncompress_update_path sender_id state.treesync_state.tree path in
         let treesync_path = update_path_to_treesync uncompressed_path in
-        treekem_path <-- update_path_to_treekem group_context_bytes uncompressed_path;
-        commit_pend <-- MLS.TreeSync.API.prepare_commit state.treesync_state treesync_path;
+        let? treekem_path = update_path_to_treekem group_context_bytes uncompressed_path in
+        let? commit_pend = MLS.TreeSync.API.prepare_commit state.treesync_state treesync_path in
         // TODO AS check
         let treesync_state = MLS.TreeSync.API.finalize_commit commit_pend () in
         let treekem_state = MLS.TreeKEM.API.commit state.treekem_state treekem_path in
         return ({ state with treesync_state; treekem_state;})
       )
-  );
+  ) in
   // 2. Increase epoch -- TODO when should this happen?!!
   let state = { state with epoch = state.epoch + 1 } in
   // 3. Update transcript
-  confirmation_tag <-- (match message_auth.confirmation_tag with | Some x -> return x | None -> error "process_commit: no confirmation tag");
-  confirmed_transcript_hash <-- MLS.TreeDEM.Message.Transcript.compute_confirmed_transcript_hash
-    message message_auth.signature state.interim_transcript_hash;
-  interim_transcript_hash <-- MLS.TreeDEM.Message.Transcript.compute_interim_transcript_hash
-    (confirmation_tag <: bytes) confirmed_transcript_hash;
+  let? confirmation_tag = (match message_auth.confirmation_tag with | Some x -> return x | None -> error "process_commit: no confirmation tag") in
+  let? confirmed_transcript_hash = MLS.TreeDEM.Message.Transcript.compute_confirmed_transcript_hash
+    message message_auth.signature state.interim_transcript_hash in
+  let? interim_transcript_hash = MLS.TreeDEM.Message.Transcript.compute_interim_transcript_hash
+    (confirmation_tag <: bytes) confirmed_transcript_hash in
   let state = { state with confirmed_transcript_hash; interim_transcript_hash } in
   // 4. New group context
-  group_context <-- state_to_group_context state;
+  let? group_context = state_to_group_context state in
   // 5. Ratchet.
-  init_secret <-- MLS.TreeDEM.Keys.secret_epoch_to_init state.epoch_secret;
-  leaf_secret <-- (
+  let? init_secret = MLS.TreeDEM.Keys.secret_epoch_to_init state.epoch_secret in
+  let? leaf_secret = (
     if state.leaf_index = sender_id && (Some? message_content.c_path) then (
       match List.Tot.assoc ((ps_to_pse (ps_leaf_node_nt _)).serialize_exact (Some?.v message_content.c_path).leaf_node) state.pending_updatepath with
       | Some leaf_secret -> return leaf_secret
@@ -220,8 +220,8 @@ let process_commit state message message_auth =
     ) else (
       return state.leaf_secret
     )
-  );
-  opt_commit_secret <-- (
+  ) in
+  let? opt_commit_secret = (
     match message_content.c_path with
     | None -> return None
     | Some _ ->
@@ -229,15 +229,15 @@ let process_commit state message message_auth =
         error "process_commit: leaf index is too big"
       else (
         assume(state.treesync_state.levels == state.treekem_state.levels);
-        commit_secret <-- MLS.TreeKEM.Operations.root_secret state.treekem_state.tree state.leaf_index leaf_secret;
+        let? commit_secret = MLS.TreeKEM.Operations.root_secret state.treekem_state.tree state.leaf_index leaf_secret in
         return (Some commit_secret)
       )
-  );
+  ) in
   let serialized_group_context = (ps_to_pse ps_group_context_nt).serialize_exact group_context in
-  joiner_secret <-- MLS.TreeDEM.Keys.secret_init_to_joiner init_secret opt_commit_secret serialized_group_context;
-  epoch_secret <-- MLS.TreeDEM.Keys.secret_joiner_to_epoch joiner_secret None serialized_group_context;
+  let? joiner_secret = MLS.TreeDEM.Keys.secret_init_to_joiner init_secret opt_commit_secret serialized_group_context in
+  let? epoch_secret = MLS.TreeDEM.Keys.secret_joiner_to_epoch joiner_secret None serialized_group_context in
   let state = { state with epoch_secret; leaf_secret; pending_updatepath = [];} in
-  state <-- reset_ratchet_states state;
+  let? state = reset_ratchet_states state in
   return (state, (joiner_secret <: bytes))
 
 let fresh_key_pair e =
@@ -278,12 +278,12 @@ let default_capabilities =
 
 val fresh_key_package_internal: e:entropy { Seq.length e == 64 } -> credential -> MLS.Crypto.sign_private_key bytes -> result (key_package_nt bytes tkt & bytes)
 let fresh_key_package_internal e { identity; signature_key } private_sign_key =
-  tmp <-- chop_entropy e (kdf_length #bytes);
+  let? tmp = chop_entropy e (kdf_length #bytes) in
   let fresh, e = tmp in
   let leaf_secret = fresh in
-  key_pair <-- MLS.TreeKEM.Operations.derive_keypair_from_path_secret #bytes leaf_secret;
+  let? key_pair = MLS.TreeKEM.Operations.derive_keypair_from_path_secret #bytes leaf_secret in
   let (_, encryption_key) = key_pair in
-  capabilities <-- default_capabilities;
+  let? capabilities = default_capabilities in
   let extensions = empty_extensions #bytes #cb.base in
   cb.hpke_public_key_length_bound;
   let leaf_data: leaf_node_data_nt bytes tkt = {
@@ -296,7 +296,7 @@ let fresh_key_package_internal e { identity; signature_key } private_sign_key =
     parent_hash = ();
     extensions;
   } in
-  signature <-- (
+  let? signature = (
     let tbs = (ps_to_pse (ps_leaf_node_tbs_nt _)).serialize_exact ({
       data = leaf_data;
       group_id = ();
@@ -304,10 +304,10 @@ let fresh_key_package_internal e { identity; signature_key } private_sign_key =
     }) in
     if not (length tbs < pow2 30 && sign_with_label_pre #bytes "LeafNodeTBS" (length #bytes tbs)) then error "fresh_key_package: tbs too long"
     else (
-      nonce <-- universal_sign_nonce;
+      let? nonce = universal_sign_nonce in
       return (sign_with_label private_sign_key "LeafNodeTBS" tbs nonce)
     )
-  );
+  ) in
   sign_signature_length_bound #bytes;
   let leaf_node: leaf_node_nt bytes tkt = {
     data = leaf_data;
@@ -320,7 +320,7 @@ let fresh_key_package_internal e { identity; signature_key } private_sign_key =
     leaf_node;
     extensions = [];
   } <: key_package_tbs_nt bytes tkt) in
-  nonce <-- universal_sign_nonce;
+  let? nonce = universal_sign_nonce in
   let tbs: bytes = (ps_to_pse (ps_key_package_tbs_nt _)).serialize_exact kp_tbs in
   if not (length tbs < pow2 30 && sign_with_label_pre #bytes "KeyPackageTBS" (length #bytes tbs)) then error "fresh_key_package: tbs too long"
   else (
@@ -332,39 +332,39 @@ let fresh_key_package_internal e { identity; signature_key } private_sign_key =
   )
 
 let fresh_key_package e cred private_sign_key =
-  tmp <-- fresh_key_package_internal e cred private_sign_key;
+  let? tmp = fresh_key_package_internal e cred private_sign_key in
   let key_package, leaf_secret = tmp in
   let key_package_bytes = (ps_to_pse (ps_key_package_nt _)).serialize_exact key_package in
-  hash <-- hash_leaf_package key_package.tbs.leaf_node;
+  let? hash = hash_leaf_package key_package.tbs.leaf_node in
   return (key_package_bytes, hash, leaf_secret)
 
 let current_epoch s = s.epoch
 
 #push-options "--fuel 2 --z3rlimit 50"
 let create e cred private_sign_key group_id =
-  tmp <-- chop_entropy e 64;
+  let? tmp = chop_entropy e 64 in
   let fresh, e = tmp in
-  tmp <-- fresh_key_package_internal fresh cred private_sign_key;
+  let? tmp = fresh_key_package_internal fresh cred private_sign_key in
   let key_package, leaf_secret = tmp in
-  treesync_state <-- (
+  let? treesync_state = (
     if not (length #bytes group_id < pow2 30) then error "create: group_id too long"
     else (
-      create_pend <-- MLS.TreeSync.API.prepare_create group_id key_package.tbs.leaf_node;
+      let? create_pend = MLS.TreeSync.API.prepare_create group_id key_package.tbs.leaf_node in
       //TODO AS check
       return (MLS.TreeSync.API.finalize_create create_pend ())
     )
-  );
-  treekem <-- treesync_to_treekem treesync_state.tree;
+  ) in
+  let? treekem = treesync_to_treekem treesync_state.tree in
   let treekem_state: treekem_state bytes = { levels = treesync_state.levels; tree = treekem } in
   // 10. In principle, the above process could be streamlined by having the
   // creator directly create a tree and choose a random value for first epoch's
   // epoch secret.
-  tmp <-- chop_entropy e 32;
+  let? tmp = chop_entropy e 32 in
   let epoch_secret, e = tmp in
-  encryption_secret <-- MLS.TreeDEM.Keys.secret_epoch_to_encryption #bytes epoch_secret;
-  leaf_dem_secret <-- MLS.TreeDEM.Keys.leaf_kdf #bytes #bytes_crypto_bytes #0 #0 encryption_secret 0;
-  handshake_state <-- MLS.TreeDEM.Keys.init_handshake_ratchet leaf_dem_secret;
-  application_state <-- MLS.TreeDEM.Keys.init_application_ratchet leaf_dem_secret;
+  let? encryption_secret = MLS.TreeDEM.Keys.secret_epoch_to_encryption #bytes epoch_secret in
+  let? leaf_dem_secret = MLS.TreeDEM.Keys.leaf_kdf #bytes #bytes_crypto_bytes #0 #0 encryption_secret 0 in
+  let? handshake_state = MLS.TreeDEM.Keys.init_handshake_ratchet leaf_dem_secret in
+  let? application_state = MLS.TreeDEM.Keys.init_application_ratchet leaf_dem_secret in
   return ({
     treesync_state;
     treekem_state;
@@ -385,23 +385,23 @@ val send_helper: state -> msg:message_content bytes{msg.wire_format == WF_mls_ci
 let send_helper st msg e =
   //FIXME
   assume (sign_nonce_length #bytes == 0);
-  tmp <-- chop_entropy e 4; let (rand_reuse_guard, e) = tmp in
-  tmp <-- chop_entropy e (sign_nonce_length #bytes); let (rand_nonce, e) = tmp in
+  let? (rand_reuse_guard, e) = chop_entropy e 4 in
+  let? (rand_nonce, e) = chop_entropy e (sign_nonce_length #bytes) in
   assume(Seq.length rand_reuse_guard == length #bytes rand_reuse_guard);
   assume(Seq.length rand_nonce == length #bytes rand_nonce);
-  group_context <-- state_to_group_context st;
-  confirmation_secret <-- MLS.TreeDEM.Keys.secret_epoch_to_confirmation st.epoch_secret;
-  sender_data_secret <-- MLS.TreeDEM.Keys.secret_epoch_to_sender_data st.epoch_secret;
-  auth <-- message_compute_auth msg st.sign_private_key rand_nonce (Some group_context) confirmation_secret st.interim_transcript_hash;
-  msg_network <-- message_content_to_network msg;
-  auth_network <-- message_auth_to_network auth;
+  let? group_context = state_to_group_context st in
+  let? confirmation_secret = MLS.TreeDEM.Keys.secret_epoch_to_confirmation st.epoch_secret in
+  let? sender_data_secret = MLS.TreeDEM.Keys.secret_epoch_to_sender_data st.epoch_secret in
+  let? auth = message_compute_auth msg st.sign_private_key rand_nonce (Some group_context) confirmation_secret st.interim_transcript_hash in
+  let? msg_network = message_content_to_network msg in
+  let? auth_network = message_auth_to_network auth in
   let auth_msg: mls_authenticated_content_nt bytes = {
     wire_format = WF_mls_ciphertext();
     content = msg_network;
     auth = auth_network;
   } in
   let ratchet = if msg.content_type = CT_application () then st.application_state else st.handshake_state in
-  ct_new_ratchet_state <-- message_to_message_ciphertext ratchet rand_reuse_guard sender_data_secret auth_msg;
+  let? ct_new_ratchet_state = message_to_message_ciphertext ratchet rand_reuse_guard sender_data_secret auth_msg in
   let (ct, new_ratchet_state) = ct_new_ratchet_state in
   let msg_bytes = (ps_to_pse ps_mls_message_nt).serialize_exact (M_mls10 (M_ciphertext ct)) in
   let new_st = if msg.content_type = CT_application () then { st with application_state = new_ratchet_state } else { st with handshake_state = new_ratchet_state } in
@@ -414,8 +414,8 @@ let rec unsafe_mk_randomness #l e =
   match l with
   | [] -> return (mk_empty_randomness bytes, e)
   | h::t ->
-    tmp <-- chop_entropy e h; let (rand_head, e) = tmp in
-    tmp <-- unsafe_mk_randomness #t e; let (rand_tail, e) = tmp in
+    let? (rand_head, e) = chop_entropy e h in
+    let? (rand_tail, e) = unsafe_mk_randomness #t e in
     assume(Seq.length rand_head == length #bytes rand_head);
     return (mk_randomness #bytes #_ #h (rand_head, rand_tail), e)
 #pop-options
@@ -439,7 +439,7 @@ let generate_key_package_and_path_secret future_state msg new_key_package =
       else (
         let tk = future_state.treekem_state.tree in
         assume(future_state.treesync_state.levels == future_state.treekem_state.levels);
-        path_secret <-- path_secret_at_least_common_ancestor tk future_state.leaf_index new_leaf_index future_state.leaf_secret;
+        let? path_secret = path_secret_at_least_common_ancestor tk future_state.leaf_index new_leaf_index future_state.leaf_secret in
         return (new_key_package, Some path_secret)
       )
   )
@@ -449,23 +449,23 @@ let generate_key_package_and_path_secret future_state msg new_key_package =
 
 val generate_welcome_message: state -> msg:message_content bytes{msg.content_type == CT_commit ()} -> message_auth bytes -> bool -> new_key_packages:list (key_package_nt bytes tkt) -> bytes -> result (welcome bytes)
 let generate_welcome_message st msg msg_auth include_path_secrets new_leaf_packages e =
-  tmp <-- process_commit st msg msg_auth;
+  let? tmp = process_commit st msg msg_auth in
   let (future_state, joiner_secret) = tmp in
-  confirmation_tag <-- from_option "generate_welcome_message: confirmation tag is missing" msg_auth.confirmation_tag;
-  tree_hash <-- (
+  let? confirmation_tag = from_option "generate_welcome_message: confirmation tag is missing" msg_auth.confirmation_tag in
+  let? tree_hash = (
     if not (MLS.TreeSync.TreeHash.tree_hash_pre future_state.treesync_state.tree) then
       error "generate_welcome_message: bad tree hash pre"
     else
       return #bytes (MLS.TreeSync.TreeHash.tree_hash future_state.treesync_state.tree)
-  );
-  ratchet_tree <-- treesync_to_ratchet_tree future_state.treesync_state.tree;
-  ratchet_tree_bytes <-- (
+  ) in
+  let? ratchet_tree = treesync_to_ratchet_tree future_state.treesync_state.tree in
+  let? ratchet_tree_bytes = (
     let l = bytes_length (ps_option (ps_node_nt tkt)) ratchet_tree in
     if l < pow2 30 then
       return #bytes ((ps_to_pse (ps_ratchet_tree_nt tkt)).serialize_exact ratchet_tree)
     else
       internal_failure "generate_welcome_message: ratchet_tree too big"
-  );
+  ) in
   let group_info: welcome_group_info bytes = {
     group_context = {
       version = PV_mls10 ();
@@ -481,14 +481,14 @@ let generate_welcome_message st msg msg_auth include_path_secrets new_leaf_packa
     signer = future_state.leaf_index;
     signature = empty; //Signed afterward
   } in
-  group_info <-- (
-    nonce <-- universal_sign_nonce;
+  let? group_info = (
+    let? nonce = universal_sign_nonce in
     sign_welcome_group_info future_state.sign_private_key group_info nonce
-  );
-  key_packages_and_path_secrets <-- mapM (generate_key_package_and_path_secret future_state msg) new_leaf_packages;
+  ) in
+  let? key_packages_and_path_secrets = mapM (generate_key_package_and_path_secret future_state msg) new_leaf_packages in
   assume (List.Tot.length key_packages_and_path_secrets == List.Tot.length new_leaf_packages);
-  tmp <-- unsafe_mk_randomness e; let (rand, e) = tmp in
-  welcome_msg <-- encrypt_welcome group_info joiner_secret key_packages_and_path_secrets rand;
+  let? (rand, e) = unsafe_mk_randomness e in
+  let? welcome_msg = encrypt_welcome group_info joiner_secret key_packages_and_path_secrets rand in
   return welcome_msg
 
 #push-options "--ifuel 2 --fuel 2 --z3rlimit 30"
@@ -501,41 +501,41 @@ let generate_update_path st e proposals =
   // This optimization (necessary for interop) is currently not implemented
   // It also needs to be implemented in `process_commit`.
   // This is the reason of processing the proposals here, since we need to know which leaves will be added
-  st <-- process_proposals st st.leaf_index proposals; //This will be more complex in the future, or maybe process_proposals will give the indices of new leaves?
+  let? st = process_proposals st st.leaf_index proposals in //This will be more complex in the future, or maybe process_proposals will give the indices of new leaves?
   if not (st.leaf_index < pow2 st.treesync_state.levels) then
     internal_failure "generate_update_path: leaf index is too big"
   else (
     assume(st.treesync_state.levels == st.treekem_state.levels);
     let update_path_entropy = update_path_entropy_lengths st.treekem_state.tree st.leaf_index in
-    tmp <-- unsafe_mk_randomness e; let (update_path_rand, e) = tmp in
+    let? (update_path_rand, e) = unsafe_mk_randomness e in
     let update_path_rand: randomness bytes update_path_entropy = update_path_rand in
-    tmp <-- chop_entropy e (sign_nonce_length #bytes);
+    let? tmp = chop_entropy e (sign_nonce_length #bytes) in
     let fresh, e = tmp in
     let sign_nonce = fresh in
     assume(length #bytes sign_nonce == Seq.length sign_nonce);
-    group_context <-- state_to_group_context st;
+    let? group_context = state_to_group_context st in
     let group_context_bytes = (ps_to_pse ps_group_context_nt).serialize_exact group_context in
     let new_leaf_secret = Seq.create (hpke_private_key_length #bytes) (Lib.IntTypes.u8 0)  in
     assume(length new_leaf_secret == Seq.length new_leaf_secret);
-    tmp <-- update_path st.treekem_state.tree st.leaf_index new_leaf_secret group_context_bytes update_path_rand;
+    let? tmp = update_path st.treekem_state.tree st.leaf_index new_leaf_secret group_context_bytes update_path_rand in
     let (update_path_kem, _) = tmp in
     let opt_my_leaf_package = leaf_at st.treesync_state.tree st.leaf_index in
-    my_leaf_package <-- (from_option "generate_update_path: my leaf is blanked" opt_my_leaf_package);
+    let? my_leaf_package = (from_option "generate_update_path: my leaf is blanked" opt_my_leaf_package) in
     let my_new_leaf_package_data = ({
       my_leaf_package.data with
       source = LNS_update ();
       lifetime = ();
       parent_hash = ();
     }) in
-    update_path_ext_sync <-- treekem_to_treesync my_new_leaf_package_data update_path_kem;
-    update_path_sync <-- (
+    let? update_path_ext_sync = treekem_to_treesync my_new_leaf_package_data update_path_kem in
+    let? update_path_sync = (
       if not (MLS.TreeSync.Operations.external_path_to_path_pre st.treesync_state.tree update_path_ext_sync st.treesync_state.group_id) then
         error "generate_update_path: bad precondition"
       else
         return (MLS.TreeSync.Operations.external_path_to_path st.treesync_state.tree update_path_ext_sync st.treesync_state.group_id st.sign_private_key sign_nonce)
-    );
-    uncompressed_update_path <-- mls_star_paths_to_update_path update_path_sync update_path_kem;
-    update_path <-- compress_update_path uncompressed_update_path;
+    ) in
+    let? uncompressed_update_path = mls_star_paths_to_update_path update_path_sync update_path_kem in
+    let? update_path = compress_update_path uncompressed_update_path in
     let new_key_package_bytes = (ps_to_pse (ps_leaf_node_nt tkt)).serialize_exact update_path.leaf_node in
     return (update_path, (new_key_package_bytes, new_leaf_secret), e)
   )
@@ -545,7 +545,7 @@ let message_commit = m:message_content bytes{m.wire_format == WF_mls_ciphertext 
 
 val generate_commit: state -> entropy -> list (proposal bytes) -> result (message_commit & state & entropy)
 let generate_commit state e proposals =
-  tmp <-- generate_update_path state e proposals;
+  let? tmp = generate_update_path state e proposals in
   let (update_path, pending, e) = tmp in
   let state = { state with pending_updatepath = pending::state.pending_updatepath} in
   let msg: message_content bytes = {
@@ -560,21 +560,21 @@ let generate_commit state e proposals =
   return ((msg <: message_commit), state, e)
 
 let add state key_package e =
-  kp <-- from_option "error message if it is malformed" ((ps_to_pse (ps_key_package_nt tkt)).parse_exact key_package);
+  let? kp = from_option "error message if it is malformed" ((ps_to_pse (ps_key_package_nt tkt)).parse_exact key_package) in
   let proposals = [ (Add kp) ] in
-  tmp <-- generate_commit state e proposals;
+  let? tmp = generate_commit state e proposals in
   let (msg, state, e) = tmp in
-  tmp <-- chop_entropy e 4;
+  let? tmp = chop_entropy e 4 in
   let fresh, e = tmp in
-  tmp <-- send_helper state msg fresh;
+  let? tmp = send_helper state msg fresh in
   let (state, msg_auth, g) = tmp in
-  tmp <-- chop_entropy e 32;
+  let? tmp = chop_entropy e 32 in
   let fresh, e = tmp in
   let rand = fresh in
   assume (hpke_private_key_length #bytes == 32);
   assert_norm (List.Tot.length [kp] == 1);
-  welcome_msg <-- generate_welcome_message state msg msg_auth false [kp] rand;
-  welcome_msg_network <-- welcome_to_network welcome_msg;
+  let? welcome_msg = generate_welcome_message state msg msg_auth false [kp] rand in
+  let? welcome_msg_network = welcome_to_network welcome_msg in
   let w:welcome_message = (empty #bytes, (ps_to_pse ps_welcome_nt).serialize_exact welcome_msg_network) in
   return (state, (g,w))
 
@@ -583,22 +583,22 @@ let remove state p e =
   | None -> error "remove: can't find the leaf to remove"
   | Some i -> (
     let proposals = [Remove i] in
-    tmp <-- generate_commit state e proposals;
+    let? tmp = generate_commit state e proposals in
     let (msg, state, e) = tmp in
-    tmp <-- chop_entropy e 4;
+    let? tmp = chop_entropy e 4 in
     let fresh, e = tmp in
-    tmp <-- send_helper state msg fresh;
+    let? tmp = send_helper state msg fresh in
     let (state, _, g) = tmp in
     return (state, g)
   )
 
 let update state e =
   let proposals = [] in
-  tmp <-- generate_commit state e proposals;
+  let? tmp = generate_commit state e proposals in
   let (msg, state, e) = tmp in
-  tmp <-- chop_entropy e 4;
+  let? tmp = chop_entropy e 4 in
   let fresh, e = tmp in
-  tmp <-- send_helper state msg fresh;
+  let? tmp = send_helper state msg fresh in
   let (state, _, g) = tmp in
   return (state, g)
 
@@ -612,7 +612,7 @@ let send state e data =
     content_type = CT_application ();
     content = data;
   } in
-  tmp <-- send_helper state msg e;
+  let? tmp = send_helper state msg e in
   let (new_state, msg_auth, g) = tmp in
   return (new_state, g)
 
@@ -630,9 +630,9 @@ let find_my_index #l t sign_pk =
 #push-options "--z3rlimit 50"
 let process_welcome_message w (sign_pk, sign_sk) lookup =
   let (_, welcome_bytes) = w in
-  welcome_network <-- from_option "process_welcome_message: can't parse welcome message" ((ps_to_pse ps_welcome_nt).parse_exact welcome_bytes);
+  let? welcome_network = from_option "process_welcome_message: can't parse welcome message" ((ps_to_pse ps_welcome_nt).parse_exact welcome_bytes) in
   let welcome = network_to_welcome welcome_network in
-  tmp <-- decrypt_welcome welcome (fun kp_hash ->
+  let? tmp = decrypt_welcome welcome (fun kp_hash ->
     match lookup kp_hash with
     | Some leaf_secret -> (
       //TODO: here we break result's encapsulation
@@ -641,19 +641,19 @@ let process_welcome_message w (sign_pk, sign_sk) lookup =
       | _ -> None
     )
     | None -> None
-  ) None;
+  ) None in
   let (group_info, secrets) = tmp in
-  group_id <-- (
+  let? group_id = (
     if not (length group_info.group_context.group_id < pow2 30) then
       internal_failure "process_welcome_message: group_id too long"
     else
       return #(mls_bytes bytes) group_info.group_context.group_id
-  );
-  ratchet_tree <-- from_option "bad ratchet tree" ((ps_to_pse #bytes (ps_ratchet_tree_nt tkt)).parse_exact group_info.extensions);
-  l <-- ratchet_tree_l ratchet_tree;
-  treesync_state <-- (
-    treesync <-- ratchet_tree_to_treesync l 0 ratchet_tree;
-    welcome_pend <-- MLS.TreeSync.API.prepare_welcome group_id treesync;
+  ) in
+  let? ratchet_tree = from_option "bad ratchet tree" ((ps_to_pse #bytes (ps_ratchet_tree_nt tkt)).parse_exact group_info.extensions) in
+  let? l = ratchet_tree_l ratchet_tree in
+  let? treesync_state = (
+    let? treesync = ratchet_tree_to_treesync l 0 ratchet_tree in
+    let? welcome_pend = MLS.TreeSync.API.prepare_welcome group_id treesync in
     // TODO AS check
     let const_unit _ = () in
     let tokens = List.Tot.map (Option.mapTot const_unit) welcome_pend.as_inputs in
@@ -661,27 +661,27 @@ let process_welcome_message w (sign_pk, sign_sk) lookup =
     assert(List.Tot.length tokens == pow2 l);
     FStar.Classical.forall_intro (MLS.MiscLemmas.index_map (Option.mapTot const_unit) welcome_pend.as_inputs);
     return (MLS.TreeSync.API.finalize_welcome welcome_pend tokens)
-  );
+  ) in
   let treesync = treesync_state.tree in
   let l = treesync_state.levels in
-  _ <-- ( //Check signature
-    group_info_ok <-- verify_welcome_group_info (fun leaf_ind ->
+  let? _ = ( //Check signature
+    let? group_info_ok = verify_welcome_group_info (fun leaf_ind ->
       if not (leaf_ind < pow2 l) then
         error "process_welcome_message: leaf_ind too big"
       else (
-        sender_leaf_package <-- from_option "process_welcome_message: signer leaf is blanked (1)" (leaf_at treesync leaf_ind);
+        let? sender_leaf_package = from_option "process_welcome_message: signer leaf is blanked (1)" (leaf_at treesync leaf_ind) in
         let result = sender_leaf_package.data.signature_key in
         if not (length #bytes result = sign_public_key_length #bytes) then
           error "process_welcome_message: bad public key length"
         else
           return (result <: sign_public_key bytes)
       )
-    ) group_info;
+    ) group_info in
     return ()
-  );
-  leaf_index <-- find_my_index treesync sign_pk;
-  treekem <-- (
-    treekem <-- treesync_to_treekem treesync;
+  ) in
+  let? leaf_index = find_my_index treesync sign_pk in
+  let? treekem = (
+    let? treekem = treesync_to_treekem treesync in
     match secrets.path_secret with
     | None -> return treekem
     | Some path_secret ->
@@ -691,24 +691,24 @@ let process_welcome_message w (sign_pk, sign_sk) lookup =
       else if not (signer_index < pow2 l) then
         error "process_welcome_message: signer index is too big"
       else (
-        update_path_kem <-- mk_init_path treekem leaf_index signer_index path_secret (empty #bytes);
+        let? update_path_kem = mk_init_path treekem leaf_index signer_index path_secret (empty #bytes) in
         return (MLS.TreeKEM.Operations.tree_apply_path treekem update_path_kem)
       )
-  );
-  interim_transcript_hash <-- MLS.TreeDEM.Message.Transcript.compute_interim_transcript_hash group_info.confirmation_tag group_info.group_context.confirmed_transcript_hash;
-  group_context <-- compute_group_context group_info.group_context.group_id group_info.group_context.epoch treesync group_info.group_context.confirmed_transcript_hash;
-  epoch_secret <-- MLS.TreeDEM.Keys.secret_joiner_to_epoch secrets.joiner_secret None ((ps_to_pse ps_group_context_nt).serialize_exact group_context);
-  leaf_secret <-- (
+  ) in
+  let? interim_transcript_hash = MLS.TreeDEM.Message.Transcript.compute_interim_transcript_hash group_info.confirmation_tag group_info.group_context.confirmed_transcript_hash in
+  let? group_context = compute_group_context group_info.group_context.group_id group_info.group_context.epoch treesync group_info.group_context.confirmed_transcript_hash in
+  let? epoch_secret = MLS.TreeDEM.Keys.secret_joiner_to_epoch secrets.joiner_secret None ((ps_to_pse ps_group_context_nt).serialize_exact group_context) in
+  let? leaf_secret = (
     let opt_my_leaf_package = leaf_at treesync leaf_index in
     match opt_my_leaf_package with
     | None -> internal_failure "process_welcome_message: leaf index points to a blank leaf"
     | Some my_leaf_package -> (
-      kp_hash <-- hash_leaf_package my_leaf_package;
+      let? kp_hash = hash_leaf_package my_leaf_package in
       match lookup kp_hash with
       | Some leaf_secret -> return leaf_secret
       | None -> internal_failure "process_welcome_message: decrypt_welcome found my leaf package but not proccess_welcome_message"
     )
-  );
+  ) in
   let dumb_ratchet_state: MLS.TreeDEM.Keys.ratchet_state bytes = {
     secret = mk_zero_vector (kdf_length #bytes);
     generation = 0;
@@ -730,30 +730,30 @@ let process_welcome_message w (sign_pk, sign_sk) lookup =
     interim_transcript_hash;
     pending_updatepath = [];
   } in
-  st <-- reset_ratchet_states st;
+  let? st = reset_ratchet_states st in
   return(group_info.group_context.group_id, st)
 #pop-options
 
 let process_group_message state msg =
-  msg <-- from_option "process_group_message: can't parse group message"
-    ((ps_to_pse ps_mls_message_nt).parse_exact msg);
-  tmp <-- (
+  let? msg = from_option "process_group_message: can't parse group message"
+    ((ps_to_pse ps_mls_message_nt).parse_exact msg) in
+  let? tmp = (
     match msg with
     | M_mls10 (M_plaintext msg) ->
         let auth_msg = message_plaintext_to_message msg in
-        content <-- network_to_message_content auth_msg.wire_format auth_msg.content;
-        auth <-- network_to_message_auth auth_msg.auth;
+        let? content = network_to_message_content auth_msg.wire_format auth_msg.content in
+        let? auth = network_to_message_auth auth_msg.auth in
         return (content, auth)
     | M_mls10  (M_ciphertext msg) ->
-        encryption_secret <-- MLS.TreeDEM.Keys.secret_epoch_to_encryption state.epoch_secret;
-        sender_data_secret <-- MLS.TreeDEM.Keys.secret_epoch_to_sender_data state.epoch_secret;
-        auth_msg <-- message_ciphertext_to_message state.treesync_state.levels (encryption_secret <: bytes) (sender_data_secret <: bytes) msg;
-        content <-- network_to_message_content auth_msg.wire_format auth_msg.content;
-        auth <-- network_to_message_auth auth_msg.auth;
+        let? encryption_secret = MLS.TreeDEM.Keys.secret_epoch_to_encryption state.epoch_secret in
+        let? sender_data_secret = MLS.TreeDEM.Keys.secret_epoch_to_sender_data state.epoch_secret in
+        let? auth_msg = message_ciphertext_to_message state.treesync_state.levels (encryption_secret <: bytes) (sender_data_secret <: bytes) msg in
+        let? content = network_to_message_content auth_msg.wire_format auth_msg.content in
+        let? auth = network_to_message_auth auth_msg.auth in
         return (content, auth)
     | _ ->
         internal_failure "unknown message type"
-  );
+  ) in
   let message, message_auth = tmp in
   // Note: can't do a dependent pair pattern matching, have to nest matches +
   // annotations because of the dependency
@@ -768,14 +768,14 @@ let process_group_message state msg =
       let message_content: commit bytes = message.content in
       begin match message_content with
       | { c_proposals = [ Proposal (Add key_package) ]; c_path = _ } ->
-          tmp <-- process_commit state message message_auth;
+          let? tmp = process_commit state message message_auth in
           let (state, _) = tmp in
           let leaf_package = key_package.tbs.leaf_node in
-          identity <-- (
+          let? identity = (
             match leaf_package.data.credential with
             | C_basic identity -> return identity
             | _ -> error "process_group_message: unknown certificate type"
-          );
+          ) in
           return (state, MsgAdd identity)
       | _ -> internal_failure "TODO: commit (general case)"
       end
