fstar/MLS.TreeDEM.KeyPackageRef.fst
@@ -11,5 +11,5 @@ open MLS.Result
 val compute_key_package_ref: #bytes:Type0 -> {|crypto_bytes bytes|} -> key_package_nt bytes tkt -> result (key_package_ref_nt bytes)
 let compute_key_package_ref #bytes #cb kp =
   let kp_bytes: bytes = serialize (key_package_nt bytes tkt) kp in
-  res <-- make_keypackage_ref kp_bytes;
+  let? res = make_keypackage_ref kp_bytes in
   return (res <: mls_bytes bytes)
