fstar/MLS.TreeSync.IntegrityCheck.fst
@@ -95,9 +95,9 @@ let check_leaf #bytes #cb leaf_index olp group_id =
   match olp with
   | None -> return IE_Good
   | Some lp -> (
-    signature_check <-- check_signature lp group_id leaf_index;
-    capabilities_check <-- check_capabilities lp;
-    lifetime_check <-- check_lifetime lp;
+    let? signature_check = check_signature lp group_id leaf_index in
+    let? capabilities_check = check_capabilities lp in
+    let? lifetime_check = check_lifetime lp in
     let signature_either = convert_opt_leaf_error_to_either signature_check leaf_index in
     let capabilities_either = convert_opt_leaf_error_to_either capabilities_check leaf_index in
     let lifetime_either = convert_opt_leaf_error_to_either lifetime_check leaf_index in
@@ -127,22 +127,22 @@ let check_internal_node #bytes #cb #tkt #l #i t =
   match onp with
   | None -> return IE_Good
   | Some np -> (
-    parent_hash_from_left_ok <-- (
+    let? parent_hash_from_left_ok = (
       if not (compute_parent_hash_pre np.content (length #bytes np.parent_hash) (MLS.TreeSync.Invariants.ParentHash.un_add right np.unmerged_leaves)) then
         error "check_internal_node: parent hash precondition not verified"
       else (
         let computed_parent_hash = compute_parent_hash np.content np.parent_hash (MLS.TreeSync.Invariants.ParentHash.un_add right np.unmerged_leaves) in
         return (has_child_with_parent_hash left computed_parent_hash)
       )
-    );
-    parent_hash_from_right_ok <-- (
+    ) in
+    let? parent_hash_from_right_ok = (
       if not (compute_parent_hash_pre np.content (length #bytes np.parent_hash) (MLS.TreeSync.Invariants.ParentHash.un_add left np.unmerged_leaves)) then
         error "check_internal_node: parent hash precondition not verified"
       else (
         let computed_parent_hash = compute_parent_hash np.content np.parent_hash (MLS.TreeSync.Invariants.ParentHash.un_add left np.unmerged_leaves) in
         return (has_child_with_parent_hash right computed_parent_hash)
       )
-    );
+    ) in
     if (parent_hash_from_left_ok || parent_hash_from_right_ok) then
       return IE_Good
     else
@@ -155,9 +155,9 @@ val check_treesync: #bytes:Type0 -> {|crypto_bytes bytes|} -> #tkt:treekem_types
 let rec check_treesync #bytes #cb #tkt #l #i t group_id =
   match t with
   | TNode onp left right ->
-    left_ok <-- check_treesync left group_id;
-    right_ok <-- check_treesync right group_id;
-    cur_ok <-- check_internal_node t;
+    let? left_ok = check_treesync left group_id in
+    let? right_ok = check_treesync right group_id in
+    let? cur_ok = check_internal_node t in
     return (left_ok &&& cur_ok &&& right_ok)
   | TLeaf olp ->
     check_leaf i olp group_id
